\section{Well Clear}~/label{sec:wellclear}  

Overview of well clear. Probably summarize Cesar's papers on the subject.
Some basic formulas : \newline
$WCV_{t_{\mathrm{var}}} (\mathbf s,s_z,\mathbf v,v_z) \equiv \mathrm{Horizontal\_WCV_\mathit{t_{\mathrm{var}}}}(\mathbf{s},\mathbf v) ~\mathrm{and}~ \mathrm{Vertical\_WCV}(s_z,v_z)$ \newline
$\mathrm{Horizontal\_WCV_\mathit{t_{\mathrm{var}}}}(\mathbf{s},\mathbf v) \equiv \Vert \mathbf s \Vert \leq \mathrm{DTHR} ~ \mathrm{or} ~ 
(d_{\mathrm{cpa}}(\mathbf s, \mathbf v)  \leq \mathrm{DTHR} ~ \mathrm{and} ~ 0 \leq t_{\mathrm{var}}(\mathbf s, \mathbf v) \leq \mathrm{TTHR})$\newline
$\mathrm{Vertical\_WCV}(s_z,v_z) \equiv \vert s_z \vert \leq \mathrm{ZTHR} ~\mathrm{or}~ 0 \leq t_{\mathrm{coa}}(s_z,v_z) \leq \mathrm{TCOA}$\newline
$d_{\mathrm{cpa}} (\mathbf s, \mathbf v) = \Vert \mathbf s + t_{\mathrm{cpa}}(\mathbf s, \mathbf v) \mathbf v \Vert$ \newline
$t_{\mathrm{coa}}(s_z,v_z) \equiv \left\{
\begin{array}{ll}
- \frac{s_z}{v_z} & \mathrm{if} ~ {s_z}{v_z} < 0\\
- 1  & \mathrm{otherwise}
\end{array}
\right. $ \newline 
\newline 

With : \newline 
$\tau(\mathbf{s},\mathbf v) \equiv \left\{
\begin{array}{ll}
- \frac{\mathbf{s}^2}{\mathbf{s} \cdot \mathbf{v}} & \mathrm{if} ~ \mathbf{s} \cdot \mathbf{v} < 0\\
- 1  & \mathrm{otherwise}
\end{array}
\right. $\newline 
$t_{\mathrm{cpa}}(\mathbf{s},\mathbf v) \equiv \left\{
\begin{array}{ll}
- \frac{\mathbf{s} \cdot \mathbf{v}}{\mathbf{v}^2} & \mathrm{if} ~ \mathbf{v} \neq 0\\
0  & \mathrm{otherwise}
\end{array}
\right. $\newline 
$\tau_{\mathrm{mod}}(\mathbf{s},\mathbf v) \equiv \left\{
\begin{array}{ll}
\frac{\mathrm{DTHR}^2-\mathbf{s}^2}{\mathbf{s} \cdot \mathbf{v}} & \mathrm{if} ~ \mathbf{s} \cdot \mathbf{v} < 0\\
-1  & \mathrm{otherwise}
\end{array}
\right. $ \newline
$t_{\mathrm{ep}}(\mathbf{s},\mathbf v) \equiv \left\{
\begin{array}{ll}
\Theta (\mathbf{s},\mathbf{v}, \mathrm{DTHR}, -1) & \mathrm{if} ~ \mathbf{s} \cdot \mathbf{v} < 0 ~\mathrm{and}~ \Delta(\mathbf{s},\mathbf v, \mathrm{DTHR}) \ge 0\\
-1  & \mathrm{otherwise}
\end{array}
\right. $ \newline
$\Theta (\mathbf{s},\mathbf{v}, D, \epsilon) \equiv \frac{-\mathbf{s}\cdot\mathbf{v} + \epsilon \sqrt{\Delta(\mathbf{s},\mathbf{v},D)}}{\mathbf{v}^2}$\newline
$\Delta(\mathbf{s},\mathbf{v},D) \equiv D^2\mathbf{v}^2 - (\mathbf{s}\cdot\mathbf{v}^{\perp})^2 \\
\Leftrightarrow \Delta(\mathbf{s},\mathbf{v},D) \equiv D^2\mathbf{v}^2 - Det(\mathbf{s},\mathbf{v})^2$